lib/Marshalling/NLarith.i.dfy
@@ -1,0 +1,19 @@
+module NLarith {
+  lemma DivLe(a: nat, b: nat)
+    requires 0 < b
+    ensures 0 <= a / b <= a
+  {
+  }
+
+  lemma MulPreservesLe(a: nat, b: nat, c: nat)
+    requires a <= b
+    ensures a * c <= b * c
+  {
+  }
+
+  lemma DistributeLeft(a: int, b: int, c: int)
+    ensures (a + b) * c == a * c + b * c
+  {
+  }
+}
+  
